Launchbury/ArityStack.thy
@@ -13,5 +13,13 @@ lemma Astack_restr_stack_below:
   "Astack (restr_stack V S) \<sqsubseteq> Astack S"
   by (induction V S rule: restr_stack.induct) auto
 
+lemma Astack_map_Dummy[simp]:
+  "Astack (map Dummy l) = 0"
+by (induction l) auto
+
+lemma Astack_append_map_Dummy[simp]:
+  "Astack S' = 0 \<Longrightarrow> Astack (S @ S') = Astack S"
+by (induction S rule: Astack.induct) auto
+
 
 end
